Several improvements including:
1) Fixed an issue in the PRF_Encryption_IND_CPA example that was causing it to take a long time to check.
2) Modified compMap, compFold, and part of the related theory so that the list has values in Type instead of Set.
3) Added some definitions and theory related to the random oracle model and additional forms of random functions.
4) Added more general arguments about collisions between lists and random values.

src/FCF/CompFold.v
@@ -11,7 +11,7 @@ Local Open Scope list_scope.
 (* Definitions for fold, map etc.   These should probably go somewhere else. *)
 
 (* Fold a computation over a list *)
-Fixpoint compFold(A B : Set)(eqd : EqDec B)(f : B -> A -> Comp B)(init : B)(ls : list A) :=
+Fixpoint compFold(A : Type)(B : Set)(eqd : EqDec B)(f : B -> A -> Comp B)(init : B)(ls : list A) :=
   match ls with
       | nil => ret init 
       | a :: ls' =>
@@ -20,14 +20,14 @@ Fixpoint compFold(A B : Set)(eqd : EqDec B)(f : B -> A -> Comp B)(init : B)(ls :
   end.
 
 (* foldBody_option is an adapter that allows you to fold a computation with signature B -> A -> Comp (option B) over a list of A, accumulating an option B. *)
-Definition foldBody_option(A B : Set)(eqd : EqDec B)(f : B -> A -> Comp (option B))(b_opt : option B)(a : A) :=
+Definition foldBody_option(A : Type)(B : Set)(eqd : EqDec B)(f : B -> A -> Comp (option B))(b_opt : option B)(a : A) :=
   match b_opt with
       | None => ret None
       | Some b =>
         f b a
   end.
 
-Definition opt_pred(A B : Set)(P : A -> B -> Prop)(opt_a : option A)(opt_b : option B) :=
+Definition opt_pred(A B : Type)(P : A -> B -> Prop)(opt_a : option A)(opt_b : option B) :=
   match opt_a with
     | Some a =>
       match opt_b with
@@ -42,7 +42,7 @@ Definition opt_pred(A B : Set)(P : A -> B -> Prop)(opt_a : option A)(opt_b : opt
   end.
 
 Theorem foldBody_option_spec : 
-  forall (A B C D: Set)(eqda : EqDec A)(eqdb : EqDec B) (c1 : A -> C -> Comp (option A)) (c2 : B -> D -> Comp (option B)) (post : A -> B -> Prop) (pre1 : A -> B -> Prop) (pre2 : C -> D -> Prop), 
+  forall (A B : Set)(C D: Type)(eqda : EqDec A)(eqdb : EqDec B) (c1 : A -> C -> Comp (option A)) (c2 : B -> D -> Comp (option B)) (post : A -> B -> Prop) (pre1 : A -> B -> Prop) (pre2 : C -> D -> Prop), 
     (forall a b c d, 
          pre1 a b -> pre2 c d -> comp_spec (opt_pred post) (c1 a c) (c2 b d)) ->
     forall opt_a opt_b c d,
@@ -82,7 +82,7 @@ Theorem compFold_option_spec :
 Qed.
 
 (* Map a computation over a list. *)
-Fixpoint compMap (A B : Set)(eqdb : EqDec B)(c : A -> Comp B)(ls : list A) : Comp (list B) :=
+Fixpoint compMap (A : Type)(B : Set)(eqdb : EqDec B)(c : A -> Comp B)(ls : list A) : Comp (list B) :=
   match ls with
       | nil => ret nil
       | a :: lsa' =>
@@ -93,7 +93,7 @@ Fixpoint compMap (A B : Set)(eqdb : EqDec B)(c : A -> Comp B)(ls : list A) : Com
 
 
 Theorem compMap_cons: 
-  forall (A B : Set)(eqdb : EqDec B) (ls : list A)(c : A -> Comp B) (a : A) x,
+  forall (A : Type)(B : Set)(eqdb : EqDec B) (ls : list A)(c : A -> Comp B) (a : A) x,
     evalDist (compMap _ c (a :: ls)) x ==
     evalDist (b <-$ c a; lsb <-$ compMap _ c ls; ret (b :: lsb)) x.
   
@@ -104,7 +104,7 @@ Theorem compMap_cons:
 Qed.
 
 Theorem compMap_nil : 
-  forall (A B : Set)(eqdb : EqDec B)(c : A -> Comp B),
+  forall (A : Type)(B : Set)(eqdb : EqDec B)(c : A -> Comp B),
     compMap _ c nil = ret nil.
 
   intuition.
@@ -120,7 +120,7 @@ Theorem list_inhabited :
 Qed.
 
 Theorem compMap_fission_eq:
-  forall (A B C D : Set){eqdb : EqDec B}{eqdd : EqDec D}{eqdc : EqDec C}(ls : list A)(f1 : A -> Comp B)(f2 : A -> Comp C)(f3 : list B -> Comp (list D))(f4 : C -> Comp D) P,
+  forall (A : Type)(B C D : Set){eqdb : EqDec B}{eqdd : EqDec D}{eqdc : EqDec C}(ls : list A)(f1 : A -> Comp B)(f2 : A -> Comp C)(f3 : list B -> Comp (list D))(f4 : C -> Comp D) P,
     (comp_spec eq (f3 nil) (ret nil)) -> 
     (forall a, comp_spec P (f1 a) (f2 a)) -> 
     (forall r1 r2 r3, P r1 r2 ->
@@ -161,7 +161,7 @@ Qed.
   
 
 Theorem compMap_map_fission_eq :
-  forall (A B C D : Set){eqdb : EqDec B}{eqdd : EqDec D}{eqdc : EqDec C}(ls : list A)(f1 : A -> Comp B)(f2 : A -> Comp C)(f3 : B -> D)(f4 : C -> D),
+  forall (A : Type)(B C D : Set){eqdb : EqDec B}{eqdd : EqDec D}{eqdc : EqDec C}(ls : list A)(f1 : A -> Comp B)(f2 : A -> Comp C)(f3 : B -> D)(f4 : C -> D),
     (forall a, comp_spec (fun b c => f3 b = f4 c)
               (f1 a) (f2 a)) -> 
     comp_spec eq (lsb <-$ compMap _ f1 ls; ret (map f3 lsb))
@@ -181,7 +181,7 @@ Qed.
 
 
 Theorem fold_map_fission_spec_eq : 
-  forall (A B C: Set)(eqdB : EqDec B)(eqdC : EqDec C) ls c init (ca : A -> Comp B) cb,
+  forall (A : Type)(B C: Set)(eqdB : EqDec B)(eqdC : EqDec C) ls c init (ca : A -> Comp B) cb,
     (forall a init, comp_spec eq (c init a) (x <-$ ca a; cb init x)) ->
     comp_spec eq (compFold _ c init ls) 
     (lsa <-$ (compMap _ ca ls); compFold _ cb init lsa).
@@ -209,7 +209,7 @@ Theorem fold_map_fission_spec_eq :
 Qed.
 
 Theorem fold_map_fission_spec : 
-  forall (A E : Set)(P : A -> E -> Prop)(B D : Set)(eqdA : EqDec A)(c1 : A -> B -> Comp A)(ls_b : list B)(init_a : A)
+  forall (A E : Set)(P : A -> E -> Prop)(B : Type)(D : Set)(eqdA : EqDec A)(c1 : A -> B -> Comp A)(ls_b : list B)(init_a : A)
     (eqdD : EqDec D)(eqdE : EqDec E)(c2 : B -> Comp D)(c3 : E -> D -> Comp E)(init_e : E),
     P init_a init_e ->
     (forall a b e, P a e -> comp_spec P (c1 a b) (a0 <-$ c2 b; c3 e a0)) ->
@@ -410,7 +410,6 @@ Lemma list_pred_map_r_eq :
   forall (A B : Set)(ls : list A)(f : A -> B),
     list_pred (fun a b => f a = b) ls (map f ls).
   
-  
   induction ls; intuition; simpl in *.
   econstructor.
   econstructor; intuition.
@@ -460,11 +459,11 @@ Lemma list_pred_map_l_eq :
 Qed.
 
 (* map constructed out of fold -- more complicated but allows us to apply any fold theory to map operations.*)
-Definition compMap_fold (A B : Set)(eqd : EqDec B)(c : A -> Comp B)(ls : list A) :=
+Definition compMap_fold (A : Type)(B : Set)(eqd : EqDec B)(c : A -> Comp B)(ls : list A) :=
   compFold _ (fun (acc : list B)(a : A) => b <-$ c a; ret (acc ++ (b :: nil))) nil ls.
 
 Lemma compFold_spec : 
-  forall (A C D : Set)(P2 : list A -> C -> D -> Prop)(eqdc : EqDec C)(eqdd : EqDec D)(lsa : list A)(c1 : C -> A -> Comp C)(c2 : D -> A -> Comp D) init1 init2,
+  forall (A : Type)(C D : Set)(P2 : list A -> C -> D -> Prop)(eqdc : EqDec C)(eqdd : EqDec D)(lsa : list A)(c1 : C -> A -> Comp C)(c2 : D -> A -> Comp D) init1 init2,
     P2 lsa init1 init2 ->
     (forall a lsa c d, P2 (a :: lsa) c d -> comp_spec (P2 lsa) (c1 c a) (c2 d a)) ->
     comp_spec (P2 nil) (compFold _ c1 init1 lsa) (compFold _ c2 init2 lsa).
@@ -480,7 +479,7 @@ Qed.
 
 
 Theorem compMap_fold_equiv : 
-  forall (A B : Set)(eqd : EqDec B)(c : A -> Comp B)(ls : list A),
+  forall (A:Type)(B : Set)(eqd : EqDec B)(c : A -> Comp B)(ls : list A),
     comp_spec eq (compMap eqd c ls) (compMap_fold eqd c ls).
   
   induction ls; intuition; simpl.
@@ -517,7 +516,7 @@ Theorem compMap_fold_equiv :
 Qed.
 
 Lemma compFold_wf : 
-  forall (A B : Set)(eqd : EqDec A)(c : A -> B -> Comp A)(ls : list B) init,
+  forall (A : Set)(B : Type)(eqd : EqDec A)(c : A -> B -> Comp A)(ls : list B) init,
     (forall a b, well_formed_comp (c a b)) ->
     well_formed_comp (compFold _ c init ls).
   
@@ -533,7 +532,7 @@ Lemma compFold_wf :
 Qed.
 
 Lemma compMap_map : 
-  forall (A B : Set)(eqd : EqDec B)(f : A -> B) ls,
+  forall (A: Type)(B : Set)(eqd : EqDec B)(f : A -> B) ls,
     comp_spec eq (compMap _ (fun a => ret (f a)) ls) (ret (map f ls)).
   
   induction ls; intuition.
@@ -552,7 +551,7 @@ Lemma compMap_map :
 Qed.
 
 Lemma compFold_nop : 
-  forall (A B : Set)(eqd : EqDec A)(c : A -> B -> Comp A)(ls : list B) init x, 
+  forall (A: Set)(B : Type)(eqd : EqDec A)(c : A -> B -> Comp A)(ls : list B) init x, 
     In x (getSupport (compFold _ c init ls)) ->
     (forall b a, In b ls -> In a (getSupport (c init b)) -> a = init) ->
     x = init.
@@ -581,7 +580,7 @@ Lemma compFold_nop :
 Qed.
 
 Lemma compFold_app : 
-  forall (A B : Set)(eqd : EqDec A)(c : A -> B -> Comp A)(ls1 ls2 : list B) init x,
+  forall (A: Set)(B : Type)(eqd : EqDec A)(c : A -> B -> Comp A)(ls1 ls2 : list B) init x,
     evalDist (compFold _ c init (ls1 ++ ls2)) x ==
     evalDist (init' <-$ compFold _ c init ls1; compFold _ c init' ls2) x.
   
@@ -601,7 +600,7 @@ Lemma compFold_app :
 Qed.
 
 Theorem comp_fold_ext : 
-  forall (A B : Set)(eqd : EqDec A)(c1 c2 : A -> B -> Comp A)(ls : list B)(init : A),
+  forall (A B: Set)(eqd : EqDec A)(c1 c2 : A -> B -> Comp A)(ls : list B)(init : A),
     (forall a b,
        comp_spec eq (c1 a b) (c2 a b)) ->
     comp_spec eq (compFold _ c1 init ls) (compFold _ c2 init ls).
@@ -837,7 +836,7 @@ Lemma compMap_spec :
 Qed.
 
 Theorem compMap_fission_ex : 
-  forall (A B C : Set)(eqdb : EqDec B)(eqdc : EqDec C)
+  forall (A : Type)(B C : Set)(eqdb : EqDec B)(eqdc : EqDec C)
          (c1 : A -> Comp B)(c2 : B -> Comp C)(ls : list A),
     comp_spec eq 
               (compMap _ (fun a => b <-$ c1 a; c2 b) ls)
@@ -1072,7 +1071,7 @@ Lemma list_pred_allNatsLt :
 Qed.
 
 Lemma compMap_length :
-  forall (A B : Set)(eqd : EqDec B)(ls : list A) x (c : A -> Comp B) ,
+  forall (A : Type)(B : Set)(eqd : EqDec B)(ls : list A) x (c : A -> Comp B) ,
     In x (getSupport (compMap _ c ls)) ->
     length x = length ls.
   
@@ -1154,7 +1153,7 @@ Qed.
 
 
 Lemma compFold_spec' : 
-  forall (A B C D : Set)(P2 : list A -> list B -> C -> D -> Prop)(eqdc1 eqdc2  : EqDec C)(eqdd1 eqdd2 : EqDec D)(lsa : list A)(lsb : list B)(c1 : C -> A -> Comp C)(c2 : D -> B -> Comp D) init1 init2,
+  forall (A B: Type)(C D : Set)(P2 : list A -> list B -> C -> D -> Prop)(eqdc1 eqdc2  : EqDec C)(eqdd1 eqdd2 : EqDec D)(lsa : list A)(lsb : list B)(c1 : C -> A -> Comp C)(c2 : D -> B -> Comp D) init1 init2,
     length lsa = length lsb ->
     P2 lsa lsb init1 init2 ->
     (forall a lsa b lsb c d, P2 (a :: lsa) (b :: lsb) c d -> comp_spec (P2 lsa lsb) (c1 c a) (c2 d b)) ->
@@ -1177,7 +1176,7 @@ Qed.
   
 
 Lemma compMap_support_app : 
-  forall (A B : Set)(eqd : EqDec B)(c : A -> Comp B)(lsa1 lsa2 : list A)(lsb1 lsb2 : list B),
+  forall (A: Type)(B : Set)(eqd : EqDec B)(c : A -> Comp B)(lsa1 lsa2 : list A)(lsb1 lsb2 : list B),
     In lsb1 (getSupport (compMap _ c lsa1)) ->
     In lsb2 (getSupport (compMap _ c lsa2)) ->
     In (lsb1 ++ lsb2) (getSupport (compMap _ c (lsa1 ++ lsa2))).
@@ -1217,7 +1216,7 @@ Lemma list_pred_single :
 Qed.
 
 Lemma flatten_map_eq : 
-  forall (A B : Set)(ls : list (list A))(f : A -> B),
+  forall (A B : Type)(ls : list (list A))(f : A -> B),
     map f (flatten ls) = flatten (map (fun ls' => map f ls') ls).
   
   induction ls; intuition; simpl in *.
@@ -1293,7 +1292,7 @@ Lemma flatten_map_pair_eq :
 Qed.
 
 Lemma compMap_app : 
-  forall (A B : Set)(eqd : EqDec B)(ls1 ls2 : list A)(c : A -> Comp B) x,
+  forall (A: Type)(B : Set)(eqd : EqDec B)(ls1 ls2 : list A)(c : A -> Comp B) x,
     evalDist (compMap _ c (ls1 ++ ls2)) x ==
     evalDist (r1 <-$ compMap _ c ls1; r2 <-$ compMap _ c ls2; ret (r1 ++ r2)) x.
   
@@ -1327,7 +1326,7 @@ Lemma compMap_app :
 Qed.
 
 Lemma compMap_flatten :
-  forall (A B : Set)(eqd : EqDec B)(c : A -> Comp B)(ls : list (list A)),
+  forall (A: Type)(B : Set)(eqd : EqDec B)(c : A -> Comp B)(ls : list (list A)),
     comp_spec
       (fun ls1 ls2 => ls2 = flatten ls1)
       (compMap _ (fun ls' => compMap _ c ls') ls)
@@ -1357,7 +1356,7 @@ Lemma compMap_flatten :
 Qed.
 
 Lemma map_f_equal : 
-  forall (A B : Set)(f1 f2 : A -> B)(ls1 ls2 : list A),
+  forall (A B : Type)(f1 f2 : A -> B)(ls1 ls2 : list A),
     (forall a, f1 a = f2 a) ->
     ls1 = ls2 ->
     map f1 ls1 = map f2 ls2.
@@ -2068,7 +2067,7 @@ Lemma list_pred_flatten_both :
 Qed.
 
 Theorem compMap_wf :
-  forall (A B : Set){eqdb : EqDec B}(c : A -> Comp B)(ls : list A),
+  forall (A : Type)(B : Set){eqdb : EqDec B}(c : A -> Comp B)(ls : list A),
     (forall a, In a ls -> well_formed_comp (c a)) ->
     well_formed_comp (compMap _ c ls).
 
@@ -2127,7 +2126,7 @@ Theorem compFold_cons :
 Qed.
 
 Theorem compFold_support_h : 
-  forall (A B : Set)(eqda : EqDec A)(P : A -> list B -> list B -> Prop)(c : A -> B -> Comp A) (ls1 ls2 ls3 : list B)(a z : A),
+  forall (A: Set)(B : Type)(eqda : EqDec A)(P : A -> list B -> list B -> Prop)(c : A -> B -> Comp A) (ls1 ls2 ls3 : list B)(a z : A),
     In z (getSupport (compFold _ c a ls1)) ->
     P a ls2 (ls1 ++ ls3) ->
     (forall a1 a2 b ls1 ls2,
@@ -2161,7 +2160,7 @@ Theorem compFold_support_h :
 Qed.
 
 Theorem compFold_support : 
-  forall (A B : Set)(eqda : EqDec A)(P : A -> list B -> list B -> Prop)(c : A -> B -> Comp A) (ls1 : list B)(a z : A),
+  forall (A: Set)(B : Type)(eqda : EqDec A)(P : A -> list B -> list B -> Prop)(c : A -> B -> Comp A) (ls1 : list B)(a z : A),
     In z (getSupport (compFold _ c a ls1)) ->
     P a nil ls1 ->
     (forall a1 a2 b ls1 ls2,
@@ -2193,7 +2192,7 @@ Theorem list_pred_app_both_if :
 Qed.
 
 Theorem compMap_seq_map :
-  forall (A B C : Set)(eqdc : EqDec C)(ls : list A)(f : A -> B)(c : B -> Comp C),
+  forall (A B: Type)(C : Set)(eqdc : EqDec C)(ls : list A)(f : A -> B)(c : B -> Comp C),
     comp_spec eq
               (compMap _ c (map f ls))
               (compMap _ (fun x => c (f x)) ls).
@@ -2373,7 +2372,7 @@ Lemma compMap_Repeat_close :
 Qed.
 
 Theorem compMap_head : 
-  forall (A B : Set)(eqd : EqDec B)(f : A -> Comp B)(ls : list A) x,
+  forall (A: Type)(B : Set)(eqd : EqDec B)(f : A -> Comp B)(ls : list A) x,
     (forall a, In a ls -> well_formed_comp (f a)) ->
     evalDist (ls' <-$ compMap _ f ls; ret (head ls')) x ==
     evalDist (match (head ls) with
@@ -2609,7 +2608,7 @@ Theorem Repeat_unroll_n :
 Qed.
 
 Theorem compFold_ret_eq : 
-  forall (A B : Set)(eqdb : EqDec B)(ls : list A)(f : B -> A -> B) init,
+  forall (A: Type)(B : Set)(eqdb : EqDec B)(ls : list A)(f : B -> A -> B) init,
     comp_spec eq
               (compFold _ (fun b a => ret (f b a)) init ls)
               (ret (fold_left f ls init)).
@@ -2622,7 +2621,7 @@ Theorem compFold_ret_eq :
 Qed.
 
 Theorem prob_fold_add_false_0 :
-  forall (A B : Set)(c : Comp A)(ls : list B)(P : A -> bool),
+  forall (A : Set)(B : Type)(c : Comp A)(ls : list B)(P : A -> bool),
     Pr[compFold _ (fun b _ => x <-$ c; ret b && (P x)) false ls] == 0.
   
   induction ls; intuition.
