src/FCF/ROM.v
@@ -1,0 +1,1583 @@
+
+Require Import FCF.
+Require Import FCF.PRF.
+Require Import Permutation.
+
+Set Implicit Arguments.
+
+(* Sorted random functions are useful, because they ensure the function state is eq
+when queries happen in different orders. *)
+
+Section SortedRandomFunc.
+
+  Variable A B : Set.
+  Hypothesis A_EqDec : EqDec A.
+  Hypothesis B_EqDec : EqDec B.
+  Variable leA : A -> A -> bool.
+  Hypothesis leA_trans : forall a1 a2 a3, leA a1 a2 = true -> leA a2 a3 = true -> leA a1 a3 = true.
+  Hypothesis leA_refl : forall a, leA a a = true.
+  Hypothesis leA_antisymm : forall a1 a2, leA a1 a2 = true -> leA a2 a1 = true -> a1 = a2.
+  Hypothesis leA_total : forall a1 a2, (leA a1 a2) || (leA a2 a1) = true.
+  Variable rndB : Comp B.
+
+  Fixpoint insertInOrder (ls : list (A * B))(a : A)(b : B) :=
+    match ls with
+    | nil => (a, b)::ls
+    | (a', b')::ls' => if (leA a a') 
+      then ((a, b)::ls) 
+      else (a', b')::(insertInOrder ls' a b)
+    end.
+
+  Theorem insertInOrder_twice_eq : forall (ls : list (A * B)) a1 b1 a2 b2,
+    a1 <> a2 ->
+    insertInOrder (insertInOrder ls a1 b1) a2 b2 =
+    insertInOrder (insertInOrder ls a2 b2) a1 b1.
+
+    induction ls; intuition idtac; simpl in *.
+    case_eq (leA a2 a1); intros.
+    case_eq (leA a1 a2); intros.
+    exfalso.
+    eapply H.
+    eapply leA_antisymm; eauto.
+    trivial.
+    case_eq (leA a1 a2); intros.
+    trivial.
+    specialize (leA_total a1 a2).
+    rewrite H0 in leA_total.
+    rewrite H1 in leA_total.
+    discriminate.
+    
+    case_eq (leA a1 a0); intros; 
+    case_eq (leA a2 a0); intros.
+    simpl.
+    case_eq (leA a2 a1); intros;
+    case_eq (leA a1 a2); intros.
+    exfalso.
+    eapply H.
+    eapply leA_antisymm; eauto.
+    rewrite H0.
+    trivial.
+    rewrite H1.
+    trivial.
+    specialize (leA_total a1 a2).
+    rewrite H2 in leA_total.
+    rewrite H3 in leA_total.
+    discriminate.
+    simpl.
+    rewrite H0.
+    case_eq (leA a2 a1); intros.
+    erewrite leA_trans in H1; eauto. discriminate.
+    rewrite H1.
+    trivial.
+
+    simpl.
+    rewrite H1.
+    rewrite H0.
+    case_eq (leA a1 a2); intros.
+    erewrite leA_trans in H0; eauto. discriminate.
+    trivial.
+
+    simpl.
+    rewrite H1.
+    rewrite H0.
+    f_equal.
+    eauto.
+
+  Qed.
+
+  Theorem arrayLookup_insertInOrder_same : 
+    forall (ls : list (A * B)) a b,
+    arrayLookup _ (insertInOrder ls a b) a = Some b.
+
+    induction ls; intuition idtac; simpl in *.
+    rewrite eqb_refl.
+    trivial.
+    case_eq (leA a a0); intuition idtac.
+    simpl.
+    rewrite eqb_refl.
+    trivial.
+    simpl.
+    case_eq (eqb a a0); intuition idtac.
+    rewrite eqb_leibniz in H0.
+    subst.
+    rewrite leA_refl in H.
+    discriminate.
+    eauto.
+
+  Qed.
+
+  Theorem arrayLookup_insertInOrder_ne : 
+    forall (ls : list (A * B)) a1 a2 b,
+    a1 <> a2 ->
+    arrayLookup _ (insertInOrder ls a1 b) a2 = arrayLookup _ ls a2.
+
+    induction ls; intuition idtac; simpl in *.
+    case_eq (eqb a2 a1); intuition idtac.
+    rewrite eqb_leibniz in H0.
+    subst.
+    intuition idtac.
+    case_eq (leA a1 a0); intuition idtac.
+    simpl.
+    case_eq (eqb a2 a1); intuition idtac.
+    rewrite eqb_leibniz in H1.
+    subst.
+    intuition idtac.
+    simpl.
+    case_eq (eqb a2 a0); intuition idtac.
+    eauto.
+  Qed.
+
+  Theorem insertInOrder_NoDup :
+    forall (s : list (A * B)) a b,
+    NoDup (fst (split s)) ->
+    arrayLookup _ s a = None ->
+    NoDup (fst (split (insertInOrder s a b))).
+
+    induction s; intuition idtac; simpl in *.
+    econstructor.
+    intuition idtac.
+    econstructor.
+
+    case_eq (eqb a a0); intros.
+    rewrite H1 in H0.
+    discriminate.
+    rewrite H1 in H0.
+    remember (split s) as z. destruct z.
+    simpl in *.
+    case_eq (leA a a0); intros.
+    simpl.
+    remember (split s) as z. destruct z.
+    simpl.
+    inversion H; clear H; subst.
+    econstructor.
+    simpl; intuition idtac.
+    subst.
+    rewrite eqb_refl in *.
+    discriminate.
+    eapply arrayLookup_None_not_In in H0.
+    intuition idtac.
+    rewrite <- Heqz0.
+    intuition idtac.
+    econstructor; intuition idtac.
+    pairInv.
+    intuition idtac.
+    pairInv.
+    intuition idtac.
+
+    simpl.
+    remember (split (insertInOrder s a b0)) as z. destruct z.
+    simpl.
+    inversion H; clear H; subst.
+    econstructor. 
+    assert (arrayLookup _ (insertInOrder s a b0) a0 = None).
+    rewrite arrayLookup_insertInOrder_ne.
+    eapply notInArrayLookupNone.
+    rewrite <- Heqz.
+    intuition idtac.
+    intuition idtac; subst.
+    rewrite eqb_refl in *. discriminate.
+    intuition idtac.
+    eapply arrayLookup_None_not_In in H.
+    intuition idtac.
+    rewrite <- Heqz0.
+    trivial.
+    specialize (IHs a b0).
+    intuition idtac.
+    rewrite <- Heqz0 in H3.
+    trivial.
+
+  Qed.
+
+  Definition sortedRandomFunc (ls : list (A * B))(a : A) :=
+    match (arrayLookup _ ls a) with
+    | None => b <-$ rndB; ret (b, (insertInOrder ls a b))
+    | Some b => ret (b, ls)
+  end.
+
+  Ltac matchOpt :=
+    match goal with
+    | [|- context[match ?a with | Some _ => _ | None => _ end] ] =>
+      case_eq a; intros
+    end.
+
+  Theorem sortedRandomFunc_swap : forall s d1 d2,
+    comp_spec eq
+    ([x2, s2] <-$2 sortedRandomFunc s d1; [x3, s3] <-$2 sortedRandomFunc s2 d2; ret ((x2, x3), s3))
+    ([x3, s2] <-$2 sortedRandomFunc s d2; [x2, s3] <-$2 sortedRandomFunc s2 d1; ret ((x2, x3), s3)).
+
+    intuition idtac.
+    assert B.
+    eapply comp_base_exists; eauto.
+    unfold sortedRandomFunc.
+    
+    case_eq (eqb d1 d2); intros.
+    rewrite eqb_leibniz in H0.
+    subst.
+    matchOpt.
+    fcf_simp.
+    rewrite H0.
+    fcf_simp.
+    eapply comp_spec_eq_refl.
+    fcf_inline_first.
+    fcf_skip.
+    fcf_simp.
+    rewrite arrayLookup_insertInOrder_same.
+    fcf_simp.
+    eapply comp_spec_eq_refl.
+
+    matchOpt.
+    fcf_simp.
+    matchOpt.
+    fcf_simp.
+    rewrite H1.
+    fcf_simp.
+    eapply comp_spec_ret; intuition idtac.
+    fcf_inline_first.
+    fcf_skip.
+    fcf_simp.
+    rewrite arrayLookup_insertInOrder_ne.
+    rewrite H1.
+    fcf_simp.
+    apply comp_spec_eq_refl.
+    intuition idtac; subst.
+    rewrite eqb_refl in *.
+    discriminate.
+    matchOpt.
+    fcf_simp.
+    rewrite H1.
+    fcf_inline_first.
+    fcf_skip.
+    rewrite arrayLookup_insertInOrder_ne.
+    rewrite H2.
+    fcf_simp.
+    eapply comp_spec_eq_refl.
+    intuition idtac; subst.
+    rewrite eqb_refl in *. discriminate.
+    
+    fcf_inline_first.
+    eapply (@comp_spec_eq_trans _ _ _ 
+      (a <-$ rndB; b1 <-$ rndB;
+   z <-$ ret (a, insertInOrder s d1 a);
+   [x2, s2]<-2 z;
+   z0 <-$ (
+       ret (b1, insertInOrder s2 d2 b1)); 
+      [x3, s3]<-2 z0; ret (x2, x3, s3))
+    ).
+    fcf_skip.
+    rewrite arrayLookup_insertInOrder_ne.
+    rewrite H2.
+    fcf_inline_first.
+    fcf_skip.
+    fcf_simp.
+    eapply comp_spec_eq_refl.
+    intuition idtac; subst.
+    rewrite eqb_refl in *. discriminate.
+    fcf_swap leftc.
+    fcf_skip.
+    fcf_simp.
+    rewrite arrayLookup_insertInOrder_ne.
+    rewrite H1.
+    fcf_inline_first.
+    fcf_skip.
+    fcf_simp.
+    eapply comp_spec_ret; intuition idtac.
+    f_equal.
+    eapply insertInOrder_twice_eq.
+    intuition idtac; subst.
+    rewrite eqb_refl in *; discriminate.
+    intuition idtac; subst.
+    rewrite eqb_refl in *; discriminate.
+
+  Qed.
+
+  Theorem insertInOrder_perm : forall s a b,
+    Permutation ((a, b)::s) (insertInOrder s a b).
+
+    induction s; intuition idtac; simpl in *.
+    eapply Permutation_refl.
+    case_eq (leA a a0); intros.
+    eapply Permutation_refl.
+    eapply Permutation_trans.
+    2:{
+    econstructor.
+    eapply IHs.
+    }
+    econstructor.
+
+  Qed.
+
+  Fixpoint sortDom (ls : list (A * B)) :=
+    match ls with
+    | nil => nil
+    | (d, r) :: ls' => insertInOrder (sortDom ls') d r
+    end.
+
+  Theorem sortDom_perm : forall ls,
+    Permutation ls (sortDom ls).
+
+    induction ls; intuition idtac; simpl in *.
+    econstructor.
+    eapply Permutation_trans.
+    econstructor.
+    eauto.
+    eapply insertInOrder_perm.
+
+  Qed.
+
+  Theorem arrayLookup_sortDom_eq : forall (ls : list (A * B)) a,
+    arrayLookup _ ls a = arrayLookup _ (sortDom ls) a.
+
+    induction ls; intuition idtac; simpl in *.
+    case_eq (eqb a a0); intros.
+    rewrite eqb_leibniz in H.
+    subst.
+    rewrite arrayLookup_insertInOrder_same.
+    trivial.
+    rewrite arrayLookup_insertInOrder_ne.
+    eauto.
+    intuition idtac; subst.
+    rewrite eqb_refl in *. discriminate.
+
+  Qed.
+
+  Theorem sortedRandomFunc_sorted_equiv : forall s a,
+    comp_spec (fun s1 s2 => fst s1 = fst s2 /\ (snd s2) = sortDom (snd s1))
+    (@randomFunc A B rndB _ s a) (sortedRandomFunc (sortDom s) a).
+
+    intuition idtac.
+    unfold randomFunc, sortedRandomFunc.
+    rewrite <- arrayLookup_sortDom_eq.
+    case_eq (arrayLookup A_EqDec s a); intuition idtac.
+    eapply comp_spec_ret; intuition idtac.
+    fcf_skip.
+    eapply comp_base_exists; eauto.
+    eapply comp_base_exists; eauto.
+    eapply comp_spec_ret; intuition idtac.
+
+  Qed.
+
+End SortedRandomFunc.
+
+Theorem ExpROM_swap_spec_h : forall 
+  (D1 R1 : Set)
+  (A1 : Set)
+  (c1 : OracleComp D1 R1 A1) 
+  (D2 R2 : Set)
+  (A2 : Set)
+  (c2 : OracleComp D2 R2 A2) 
+  (eqdr1 : EqDec R1)(eqdr2 : EqDec R2)
+  (eqda1 : EqDec A1)(eqda2 : EqDec A2)
+  (S : Set)(eqds : EqDec S)
+  (o1 : S -> D1 -> Comp (R1 * S))
+  (o2 : S -> D2 -> Comp (R2 * S))
+  s,
+  (forall s d1, 
+    comp_spec eq
+    ([x2, s2] <-$2 o1 s d1; [x3, s3] <-$2 c2 _ _ o2 s2; ret ((x2, x3), s3))
+    ([x3, s2] <-$2 c2 _ _  o2 s; [x2, s3] <-$2 o1 s2 d1; ret ((x2, x3), s3))
+  ) ->
+  comp_spec eq 
+  ([x2, s2] <-$2 c1 _ _ o1 s; [x3, s3] <-$2 c2 _ _ o2 s2; ret ((x2, x3), s3))
+  ([x3, s2] <-$2 c2 _ _ o2 s; [x2, s3] <-$2 c1 _ _ o1 s2; ret ((x2, x3), s3)).
+
+  induction c1; intuition idtac; simpl in *.
+
+  (* query case *)
+  specialize (@H s a).
+  despec.
+  intuition idtac.
+  exists x.
+  intuition idtac.
+
+  eapply eqRat_trans.
+  2:{
+  eapply eqRat_trans.
+  eapply H0. 
+  unfold marginal_l.
+  fcf_skip.
+  eapply evalDist_ret_eq.
+  simpl.
+  case_eq (eqbPair (pair_EqDec eqda1 eqda2) eqds
+  (fst x0) (a1, b0, b)); intros.
+  case_eq (eqbPair (pair_EqDec eqdr1 eqda2) eqds
+  (fst x0) (a1, b0, b));
+  intros.
+  eauto.
+  apply eqbPair_prop in H3.
+  destruct x0; simpl in *; subst.
+  rewrite eqbPair_refl in H4.
+  discriminate.
+  case_eq (eqbPair (pair_EqDec eqdr1 eqda2) eqds
+  (fst x0) (a1, b0, b));
+  intros.
+  apply eqbPair_prop in H4.
+  destruct x0; simpl in *; subst.
+  rewrite eqbPair_refl in H3.
+  discriminate.
+  trivial.
+  }
+  fcf_skip.
+  fcf_simp.
+  fcf_skip.
+  fcf_simp.
+  fcf_compute.
+
+  eapply eqRat_trans.
+  2:{
+  eapply eqRat_trans.
+  eapply H. 
+  unfold marginal_r.
+  fcf_skip.
+  eapply evalDist_ret_eq.
+  simpl.
+  case_eq (eqbPair (pair_EqDec eqda1 eqda2) eqds
+  (snd x0) (a1, b0, b)); intros.
+  case_eq (eqbPair (pair_EqDec eqdr1 eqda2) eqds
+  (snd x0) (a1, b0, b));
+  intros.
+  eauto.
+  apply eqbPair_prop in H3.
+  destruct x0; simpl in *; subst.
+  rewrite eqbPair_refl in H4.
+  discriminate.
+  case_eq (eqbPair (pair_EqDec eqdr1 eqda2) eqds
+  (snd x0) (a1, b0, b));
+  intros.
+  apply eqbPair_prop in H4.
+  destruct x0; simpl in *; subst.
+  rewrite eqbPair_refl in H3.
+  discriminate.
+  trivial.
+  }
+  fcf_skip.
+  fcf_simp.
+  fcf_skip.
+  fcf_simp.
+  fcf_compute.
+
+  (* run case *)
+  assert (A -> B * S) as bs.
+  intros.
+  eapply oc_base_exists; eauto.
+  intuition idtac.
+  assert (B' * S0).
+  eapply comp_base_exists; eauto.
+  intuition idtac.
+
+  assert C as c.
+  eapply oc_base_exists; eauto.
+  intuition idtac.
+
+  assert (D2 -> R2) as r2.
+  intuition idtac.
+  assert (R2 * S0).
+  eapply comp_base_exists; eauto.
+  intuition idtac.
+
+  assert A2 as a2.
+  eapply oc_base_exists; eauto.
+
+  fcf_inline_first.
+  assert (EqDec C).
+  eapply EqDec_pair_l; eauto.
+
+  eapply (@comp_spec_eq_trans_l _ _ _ _ _
+    (y <-$ (a <-$
+   c1 (S * S0)%type (pair_EqDec e eqds)
+     (fun (x : S * S0) (y : A) =>
+      p <-$ (o (fst x) y) S0 eqds o1 (snd x);
+      ret (fst (fst p), (snd (fst p), snd p))) 
+     (s, s0);
+   [x2, s3]<-2 a;
+   z0 <-$ c2 (S * S0)%type _ 
+    (fun p d => r <-$ o2 (snd p) d; ret (fst r, (fst p, snd r))) s3; 
+  [x3, s4]<-2 z0; ret (x2, x3, s4));
+  ret (((fst (fst y), fst (snd y)), (snd (fst y))), (snd (snd y))))
+  ).
+  fcf_inline_first.
+  fcf_skip.
+
+  fcf_inline_first.
+  fcf_skip.
+  simpl.
+  eapply (@fcf_oracle_eq _ _ (fun p1 p2 => p1 = (snd p2) /\ fst p2 = a));
+  intuition idtac.
+  subst.
+  eapply comp_spec_eq_trans_l.
+  eapply comp_spec_symm.
+  eapply comp_spec_consequence.
+  eapply comp_spec_right_ident.
+  intros; subst; trivial.
+  fcf_skip.
+  simpl.
+  eapply comp_spec_ret; intuition idtac.
+  simpl.
+  fcf_simp.
+  simpl in *; intuition idtac; subst.
+  eapply comp_spec_ret; intuition idtac.
+  
+  specialize (@IHc1 _ _ _ c2 _ _ _ _ (S * S0)%type _ 
+    (fun (x : S * S0) (y : A) =>
+      p <-$ (o (fst x) y) S0 eqds o1 (snd x);
+      ret (fst (fst p), (snd (fst p), snd p)))
+    (fun (p : S * S0) (d : D2) =>
+      r <-$ o2 (snd p) d; ret (fst r, (fst p, snd r)))).
+  eapply (@ comp_spec_eq_trans_r _ _ _ _ _ 
+      (y <-$ (z <-$
+          c2 _ _ 
+            (fun (p : S * S0) (d : D2) =>
+             r <-$ o2 (snd p) d; ret (fst r, (fst p, snd r))) (s, s0);
+          [x3, s3]<-2 z;
+          z0 <-$
+          c1 _ _
+            (fun (x : S * S0) (y : A) =>
+             p <-$ (o (fst x) y) S0 eqds o1 (snd x);
+             ret (fst (fst p), (snd (fst p), snd p))) s3;
+          [x2, s4]<-2 z0; ret (x2, x3, s4));
+      ret (((fst (fst y), fst (snd y)), (snd (fst y))), (snd (snd y))))
+  ).
+  eapply comp_spec_seq_eq.
+  intuition idtac.
+  intuition idtac. 
+  eapply IHc1.
+  intuition idtac.
+  simpl in *. subst.
+  eapply (@ comp_spec_eq_trans_l _ _ _ _ _ 
+    (y <-$(z <-$ (o a d1) S0 eqds o1 b;
+     [x2, s3]<-2 z;
+     z0 <-$ c2 _ _ o2 s3;
+     [x3, s4]<-2 z0; ret (x2, x3, s4));
+      ret ((fst (fst (fst y)), (snd (fst y))), (snd (fst (fst y)), (snd y)))
+    )
+  ).
+  fcf_inline_first.
+  fcf_skip.
+  simpl.
+  fcf_inline_first.
+  fcf_skip.
+  eapply (@fcf_oracle_eq _ _ (fun p1 p2 => (snd p1) = p2 /\ fst p1 = b2)); intuition idtac.
+  subst.
+  eapply comp_spec_eq_trans_r.
+  2:{
+  eapply comp_spec_right_ident.
+  }
+  fcf_skip.
+  eapply comp_spec_ret; intuition idtac.
+  fcf_simp.
+  simpl in *; intuition idtac.
+  subst.  
+  eapply comp_spec_ret; intuition idtac.
+
+  eapply (@ comp_spec_eq_trans_r _ _ _ _ _ 
+    (y <-$
+      (z <-$ c2 _ _ o2 b;
+      [x2, s3] <-2 z;
+      z0 <-$ (o a d1) _ _ o1 s3;
+      [x3, s4] <-2 z0; ret (x3, x2, s4));
+      ret ((fst (fst (fst y)), (snd (fst y))), (snd (fst (fst y)), (snd y)))
+    )
+  ).
+  eapply comp_spec_seq.
+  intuition idtac.
+  intuition idtac.
+  eapply H;
+  eauto.
+  intuition idtac.
+  subst.
+  eapply comp_spec_ret; intuition idtac.
+
+  fcf_inline_first.
+  fcf_skip.
+  eapply (@fcf_oracle_eq _ _ (fun p1 p2 => p1 = (snd p2) /\ fst p2 = a)); intuition idtac.
+  subst.
+  eapply comp_spec_eq_trans_l.
+  eapply comp_spec_symm.
+  eapply comp_spec_consequence.
+  eapply comp_spec_right_ident.
+  intros; subst; trivial.
+  fcf_skip.
+  eapply comp_spec_ret; intuition idtac.
+
+  simpl in *; intuition idtac; subst.
+  fcf_inline_first.
+  fcf_simp.
+  fcf_inline_first.
+  fcf_skip.
+  fcf_simp.
+  eapply comp_spec_eq_refl.
+
+  intros.
+  eapply comp_spec_eq_refl.
+
+  fcf_inline_first.
+  fcf_skip.
+  eapply (@fcf_oracle_eq _ _ (fun p1 p2 => snd p1 = p2 /\ fst p1 = s));
+  intuition idtac.
+  subst.
+  simpl.
+  eapply comp_spec_eq_trans_r.
+  2:{
+  eapply comp_spec_right_ident.
+  }
+  fcf_skip.
+  eapply comp_spec_ret; simpl in *; intuition idtac.
+  simpl in *; intuition idtac; subst.
+  fcf_simp.
+  fcf_inline_first.
+  fcf_skip.
+  simpl.
+  fcf_simp.
+  eapply comp_spec_ret; intuition idtac.
+
+  (* ret case *)
+  assert C as c_ex.
+  eapply comp_base_exists; eauto.
+
+  assert A2 as a2_ex.
+  eapply oc_base_exists; eauto.
+  intuition idtac.
+  assert (R2 * S).
+  eapply comp_base_exists; eauto.
+  intuition idtac.
+
+  fcf_inline_first.
+  eapply (@comp_spec_eq_trans_l _ _ _ _ _
+    (a <-$ c;
+      z0 <-$ c2 S eqds o2 s; [x3, s4]<-2 z0; ret (a, x3, s4))
+  ).
+  fcf_skip.
+  fcf_swap leftc.
+  fcf_skip.
+  fcf_inline_first.
+  fcf_skip.
+  fcf_simp.
+  eapply comp_spec_ret; intuition idtac.
+
+  (* bind case *)
+  assert C as c_ex.
+  eapply oc_base_exists; eauto.
+  intuition idtac.
+  assert (B * S).
+  eapply comp_base_exists; eauto.
+  intuition idtac.
+
+  assert C' as c'_ex.
+  eapply oc_base_exists.
+  eapply o.
+  intuition idtac.
+  intuition idtac.
+  assert (B * S).
+  eapply comp_base_exists; eauto.
+  intuition idtac.
+
+  assert A2 as a2_ex.
+  eapply oc_base_exists; eauto.
+  intuition idtac.
+  assert (R2 * S).
+  eapply comp_base_exists; eauto.
+  intuition idtac.
+
+  fcf_inline_first. 
+  eapply (@comp_spec_eq_trans_l _ _ _ _ _ 
+    (a <-$ c1 S eqds o1 s;
+     [z, s']<-2 a;
+     z <-$ ((o z) S eqds o1 s');
+     [x2, s3]<-2 z;
+     z0 <-$ c2 S eqds o2 s3;
+     [x3, s4]<-2 z0; ret (x2, x3, s4))
+  ).
+  fcf_skip.
+
+  eapply (@comp_spec_eq_trans _ _ _
+    (a <-$ c1 S eqds o1 s;
+     [z, s']<-2 a;
+     z1 <-$ c2 S eqds o2 s';
+     [x2, s3]<-2 z1;
+     z0 <-$ ((o z) S eqds o1 s3);
+     [x3, s4]<-2 z0; ret (x3, x2, s4))
+  ).
+  fcf_skip.
+  eapply H; intuition idtac.
+
+  eapply (@comp_spec_eq_trans_l _ _ _ _ _ 
+    (y <-$ (a <-$ c1 S eqds o1 s;
+     [z, s']<-2 a;
+     z1 <-$ c2 S eqds o2 s';
+     [x2, s3]<-2 z1;
+      ret (z, x2, s3)
+    );
+    z0 <-$ (o (fst (fst y))) S eqds o1 (snd y);
+     [x3, s4]<-2 z0; ret (x3, (snd (fst y)), s4))
+  ).
+  fcf_inline_first.
+  fcf_skip.
+  fcf_inline_first.
+  fcf_skip.
+  fcf_simp.
+  simpl. 
+  fcf_inline_first.
+  eapply comp_spec_eq_refl.
+
+  eapply (@comp_spec_eq_trans_r _ _ _ _ _
+    (y <-$ 
+     (a <-$ c2 S eqds o2 s;
+     [z, s']<-2 a;
+     z1 <-$ c1 S eqds o1 s';
+     [x2, s3]<-2 z1;
+      ret (x2, z, s3)
+    );
+    z0 <-$ (o (fst (fst y))) S eqds o1 (snd y);
+     [x3, s4]<-2 z0; ret (x3, (snd (fst y)), s4))
+  ).
+  eapply comp_spec_seq.
+  intuition idtac.
+  intuition idtac.
+  eapply IHc1; intuition idtac.
+  intuition idtac.
+  subst.
+  fcf_skip.
+
+  fcf_inline_first.
+  fcf_skip.
+  fcf_inline_first.
+  fcf_skip.
+  simpl.
+  fcf_skip.
+
+  Unshelve.
+
+  eapply pair_EqDec; intuition idtac.
+  eapply oc_EqDec.
+  eauto.
+  intuition idtac.
+  assert (B * S).
+  eapply comp_base_exists; eauto.
+  intuition idtac.
+  intuition idtac.
+  
+  eapply pair_EqDec; intuition idtac.
+  eapply oc_EqDec.
+  eauto.
+  intuition idtac.
+  assert (B * S).
+  eapply comp_base_exists; eauto.
+  intuition idtac.
+  intuition idtac.
+
+  eapply pair_EqDec; intuition idtac.
+  eapply oc_EqDec.
+  eauto.
+  intuition idtac.
+  assert (B * S).
+  eapply comp_base_exists; eauto.
+  intuition idtac.
+  intuition idtac.
+
+  eapply oc_EqDec.
+  eauto.
+  intuition idtac.
+  assert (B * S).
+  eapply comp_base_exists; eauto.
+  intuition idtac.
+  intuition idtac.
+
+  eapply pair_EqDec; intuition idtac.
+  eapply oc_EqDec.
+  eauto.
+  intuition idtac.
+  assert (B * S).
+  eapply comp_base_exists; eauto.
+  intuition idtac.
+  intuition idtac.
+
+Qed.
+
+Theorem ExpROM_query_swap_spec : forall 
+  (D2 R2 : Set)
+  (A2 : Set)
+  (c2 : OracleComp D2 R2 A2) 
+  (D1 R1 : Set)
+  (A1 : Set)
+  (eqdr1 : EqDec R1)(eqdr2 : EqDec R2)
+  (eqda1 : EqDec A1)(eqda2 : EqDec A2)
+  (S : Set)(eqds : EqDec S)
+  (o1 : S -> D1 -> Comp (R1 * S))
+  (o2 : S -> D2 -> Comp (R2 * S))
+  s d,
+  (forall s d1 d2, 
+    comp_spec eq
+    ([x2, s2] <-$2 o1 s d1; [x3, s3] <-$2 o2 s2 d2; ret ((x2, x3), s3))
+    ([x3, s2] <-$2 o2 s d2; [x2, s3] <-$2 o1 s2 d1; ret ((x2, x3), s3))
+  ) ->
+  comp_spec eq 
+  ([x2, s2] <-$2 o1 s d; [x3, s3] <-$2 c2 _ _ o2 s2; ret ((x2, x3), s3))
+  ([x3, s2] <-$2 c2 _ _ o2 s; [x2, s3] <-$2 o1 s2 d; ret ((x2, x3), s3)).
+
+  induction c2; intuition idtac; simpl in *.
+
+  (* query case *)
+  specialize (@H s d a).
+  despec.
+  intuition idtac.
+  exists x.
+  intuition idtac.
+
+  eapply eqRat_trans.
+  2:{
+  eapply eqRat_trans.
+  eapply H0. 
+  unfold marginal_l.
+  fcf_skip.
+  eapply evalDist_ret_eq.
+  simpl.
+  case_eq (eqbPair (pair_EqDec eqdr1 eqda2) eqds
+  (fst x0) (a1, b0, b)); intros.
+  case_eq (eqbPair (pair_EqDec eqdr1 eqdr2) eqds
+  (fst x0) (a1, b0, b));
+  intros.
+  eauto.
+  apply eqbPair_prop in H3.
+  destruct x0; simpl in *; subst.
+  rewrite eqbPair_refl in H4.
+  discriminate.
+  case_eq (eqbPair (pair_EqDec eqdr1 eqdr2) eqds
+  (fst x0) (a1, b0, b));
+  intros.
+  apply eqbPair_prop in H4.
+  destruct x0; simpl in *; subst.
+  rewrite eqbPair_refl in H3.
+  discriminate.
+  trivial.
+  }
+  fcf_skip.
+  fcf_simp.
+  fcf_skip.
+  fcf_simp.
+  fcf_compute.
+
+  eapply eqRat_trans.
+  2:{
+  eapply eqRat_trans.
+  eapply H. 
+  unfold marginal_r.
+  fcf_skip.
+  eapply evalDist_ret_eq.
+  simpl.
+  case_eq (eqbPair (pair_EqDec eqdr1 eqda2) eqds
+  (snd x0) (a1, b0, b)); intros.
+  case_eq (eqbPair (pair_EqDec eqdr1 eqdr2) eqds
+  (snd x0) (a1, b0, b));
+  intros.
+  eauto.
+  apply eqbPair_prop in H3.
+  destruct x0; simpl in *; subst.
+  rewrite eqbPair_refl in H4.
+  discriminate.
+  case_eq (eqbPair (pair_EqDec eqdr1 eqdr2) eqds
+  (snd x0) (a1, b0, b));
+  intros.
+  apply eqbPair_prop in H4.
+  destruct x0; simpl in *; subst.
+  rewrite eqbPair_refl in H3.
+  discriminate.
+  trivial.
+  }
+  fcf_skip.
+  fcf_simp.
+  fcf_skip.
+  fcf_simp.
+  fcf_compute.
+
+  (* run case *)
+
+  assert R1 as r1_ex.
+  assert (R1 * S0).
+  eapply comp_base_exists.
+  eauto.
+  intuition idtac.
+
+  assert (A' -> B') as b'_ex.
+  intros.
+  assert (B' * S0).
+  eapply comp_base_exists; eauto.
+  intuition idtac.
+
+  assert (A -> B) as b_ex.
+  intros.
+  assert (B * S).
+  eapply oc_base_exists.
+  eapply o.
+  trivial.
+  trivial.
+  trivial.
+  intuition idtac.
+  
+  assert C as c_ex.
+  eapply oc_base_exists.
+  eauto.
+  intuition idtac.
+
+  fcf_inline_first.
+  assert (EqDec C).
+  eapply EqDec_pair_l; eauto.
+
+  eapply (@comp_spec_eq_trans_l _ _ _ _ _
+    (y <-$ (z <-$ (fun p d => r <-$ o1 (snd p) d; ret (fst r, (fst p, snd r))) (s, s0) d;
+     [x2, s2]<-2 z;
+      z0 <-$
+        c2 (S * S0)%type (pair_EqDec e eqds)
+          (fun (x : S * S0) (y : A) =>
+           p <-$
+           (o (fst x) y) S0 eqds o2 (snd x);
+           ret (fst (fst p),
+               (snd (fst p), snd p))) 
+          s2;
+      [x3, s3]<-2 z0;
+      ret (x2, x3, s3));
+     ret ((fst (fst y)), (snd (fst y), fst (snd y)), snd (snd y)))
+  ).
+  fcf_inline_first.
+  fcf_skip.
+  fcf_simp.
+  fcf_inline_first.
+  fcf_skip.
+  fcf_simp.
+  eapply comp_spec_ret; intuition idtac.
+  
+  specialize (@IHc2 _ _ _ _ _ _ _ (S * S0)%type _ 
+    (fun p d => r <-$ o1 (snd p) d; ret (fst r, (fst p, snd r)))
+    (fun (x : S * S0) (y : A) =>
+       p <-$
+       (o (fst x) y) S0 eqds o2 (snd x);
+       ret (fst (fst p),
+           (snd (fst p), snd p)))
+  ).
+  eapply (@comp_spec_eq_trans_r _ _ _ _ _
+    (y <-$
+   (z <-$
+          c2 (S * S0)%type
+            (pair_EqDec e eqds)
+            (fun (x : S * S0) (y : A) =>
+             p <-$
+             (o (fst x) y) S0 eqds o2
+               (snd x);
+             ret (fst (fst p),
+                 (snd (fst p), snd p))) (s, s0);
+          [x3, s2]<-2 z;
+          z0 <-$
+          (fun (p : S * S0) (d0 : D1) =>
+           r <-$ o1 (snd p) d0;
+           ret (fst r, (fst p, snd r))) s2 d;
+          [x2, s3]<-2 z0; ret (x2, x3, s3));
+   ret (fst (fst y),
+       (snd (fst y), fst (snd y)),
+       snd (snd y)))
+  ).
+  eapply comp_spec_seq.
+  intuition idtac.
+  intuition idtac.
+  eapply IHc2.
+  
+  intuition idtac.
+  
+  simpl.
+  eapply (@comp_spec_eq_trans_l _ _ _ _ _
+      ([a, b, c] <-$3 (r <-$ o1 b d1; 
+      [x2, s2] <-2 r;
+      z0 <-$ (o a d2) S0 eqds o2 s2;
+      [x3, s3]<-2 z0; 
+      ret (x2, x3, s3));
+      ret (a, (fst b), (snd b, c)))
+  ).
+  fcf_inline_first.
+  fcf_skip.
+  fcf_inline_first.
+  simpl.
+  fcf_skip.
+  fcf_simp.
+  eapply comp_spec_ret; intuition idtac.
+
+  eapply (@comp_spec_eq_trans_r _ _ _ _ _
+    ([a, b, c] <-$3 
+      (z <-$ (o a d2) S0 eqds o2 b;
+       [x3, s2]<-2 z;
+       z0 <-$ o1 s2 d1;
+       [x2, s3]<-2 z0; ret (x2, x3, s3));
+    ret (a, (fst b), (snd b, c)))
+  ).
+  eapply comp_spec_seq_eq.
+  intuition idtac.
+  intuition idtac.
+  eapply H; intuition idtac.
+  eauto.
+  intuition idtac.
+  eapply comp_spec_eq_refl.
+  fcf_inline_first.
+  fcf_skip.
+  fcf_simp.
+  simpl.
+  fcf_inline_first.
+  fcf_skip.
+  fcf_simp.
+  apply comp_spec_ret; intuition idtac.
+
+  intuition idtac.
+  subst. simpl in *.  
+  eapply comp_spec_ret; intuition idtac.
+
+  fcf_inline_first.
+  fcf_skip.
+  fcf_inline_first.
+  fcf_simp.
+  fcf_skip.
+  simpl.
+  eapply comp_spec_ret; intuition idtac.
+
+  (* ret case *)
+  assert R1 as r1_ex.
+  assert (R1 * S).
+  eapply comp_base_exists; eauto.
+  intuition idtac.
+
+  assert C as c_ex.
+  apply comp_base_exists; eauto.
+
+  fcf_inline_first.
+  eapply comp_spec_eq_symm.
+  eapply (@comp_spec_eq_trans _ _ _ 
+    (a <-$ c;
+     z0 <-$ o1 s d;
+     [x2, s3]<-2 z0; ret (x2, a, s3))
+  ).
+  fcf_skip.
+  fcf_swap leftc.
+  fcf_skip.
+  fcf_inline_first.
+  fcf_skip.
+  fcf_simp.
+  eapply comp_spec_ret; intuition idtac.
+
+  (* bind case *)
+  assert R1 as r1_ex.
+  assert (R1 * S).
+  eapply comp_base_exists; eauto.
+  intuition idtac.
+
+  assert (A -> B).
+  intros.
+  assert (B * S).
+  eapply comp_base_exists; eauto.
+  intuition idtac.
+
+  assert C as c_ex.
+  eapply oc_base_exists; eauto.
+
+  assert C' as c'_ex.
+  eapply oc_base_exists.
+  eapply o. 
+  trivial.
+  intuition idtac.
+
+  fcf_inline_first. 
+  eapply (@comp_spec_eq_trans_l _ _ _ _ _ 
+    ([a, b, c] <-$3 (z <-$ o1 s d;
+      [x2, s2]<-2 z;
+      z0 <-$ c2 S eqds o2 s2;
+      [z1, s']<-2 z0; 
+      ret (x2, z1, s'));
+     z1 <-$
+     ((o b) S eqds o2 c);
+     [x3, s3]<-2 z1; ret (a, x3, s3))
+  ).
+  fcf_inline_first.
+  fcf_skip.
+  fcf_inline_first.
+  fcf_skip.
+  fcf_simp.
+  eapply comp_spec_eq_refl.
+
+  eapply (@comp_spec_eq_trans _ _ _ 
+    ([a, b, c] <-$3 
+      (z <-$ c2 S eqds o2 s;
+          [x3, s2]<-2 z;
+          z0 <-$ o1 s2 d;
+          [x2, s3]<-2 z0; ret (x2, x3, s3));
+     z1 <-$
+     ((o b) S eqds o2 c);
+     [x3, s3]<-2 z1; ret (a, x3, s3))
+  ).
+  eapply comp_spec_seq_eq.
+  intuition idtac.
+  intuition idtac.
+  eapply IHc2; intuition idtac.
+  eauto.
+  intuition idtac.
+  eapply comp_spec_eq_refl.
+  fcf_inline_first.
+  fcf_skip.
+  eapply comp_spec_eq_trans.
+  2:{
+  eapply H; intuition idtac.
+  eauto.
+  }
+  fcf_inline_first.
+  fcf_skip.
+  
+  Unshelve.
+
+  eapply pair_EqDec; intuition idtac.
+  eapply oc_EqDec.
+  eauto.
+  intuition idtac.
+  intuition idtac.
+
+  eapply oc_EqDec.
+  eauto.
+  intuition idtac.
+  intuition idtac.
+
+  eapply pair_EqDec; intuition idtac.
+  eapply oc_EqDec.
+  eauto.
+  intuition idtac.
+  intuition idtac.
+
+Qed.
+
+Theorem ExpROM_swap_spec : forall 
+  (D1 R1 : Set)
+  (A1 : Set)
+  (c1 : OracleComp D1 R1 A1) 
+  (D2 R2 : Set)
+  (A2 : Set)
+  (c2 : OracleComp D2 R2 A2) 
+  (eqdr1 : EqDec R1)(eqdr2 : EqDec R2)
+  (eqda1 : EqDec A1)(eqda2 : EqDec A2)
+  (S : Set)(eqds : EqDec S)
+  (o1 : S -> D1 -> Comp (R1 * S))
+  (o2 : S -> D2 -> Comp (R2 * S))
+  s,
+  (forall s d1 d2, 
+    comp_spec eq
+    ([x2, s2] <-$2 o1 s d1; [x3, s3] <-$2 o2 s2 d2; ret ((x2, x3), s3))
+    ([x3, s2] <-$2 o2 s d2; [x2, s3] <-$2 o1 s2 d1; ret ((x2, x3), s3))
+  ) ->
+  comp_spec eq 
+  ([x2, s2] <-$2 c1 _ _ o1 s; [x3, s3] <-$2 c2 _ _ o2 s2; ret ((x2, x3), s3))
+  ([x3, s2] <-$2 c2 _ _ o2 s; [x2, s3] <-$2 c1 _ _ o1 s2; ret ((x2, x3), s3)).
+
+  intuition idtac.
+  eapply ExpROM_swap_spec_h.
+  intuition idtac.
+  intuition idtac.
+  eapply ExpROM_query_swap_spec; intuition idtac.
+  
+  eauto.
+
+Qed.
+
+(* Experiments in the random oracle model and related theory. *)
+Section ExperimentROM.
+
+  Variable DomainRO RangeRO : Set.
+  Hypothesis DomainRO_EqDec : EqDec DomainRO.
+  Hypothesis RangeRO_EqDec : EqDec RangeRO.
+  Variable rndRange : Comp RangeRO.
+
+  Section WithProcs.
+    Variable T : Set.
+    Hypothesis T_EqDec : EqDec T.
+    Variable A : OracleComp DomainRO RangeRO T.
+    (* The experiment takes a function that calculates the result from the RO state *)
+    Variable X : Set.
+    Hypothesis X_EqDec : EqDec X.
+    Variable f : T -> list (DomainRO * RangeRO) -> X.
+
+    Definition ExpROM_gen_s s := 
+      [t, s] <-$2 A _ _ (@randomFunc DomainRO RangeRO rndRange _) s;
+      ret f t s.
+
+    Definition ExpROM_gen := ExpROM_gen_s nil.
+
+    Definition ExpROM := 
+      [t, _] <-$2 A _ _ (@randomFunc DomainRO RangeRO rndRange _) nil;
+      ret t.
+  End WithProcs.
+
+  Theorem ExpROM_gen_seq_eq : forall (A B C : Set) 
+    (eqdb : EqDec B)(eqdc : EqDec C)
+    (c1a c1b : OracleComp DomainRO RangeRO A) 
+    (c2a c2b : A -> OracleComp DomainRO RangeRO B) 
+    (f : B -> (list (DomainRO*RangeRO)) -> C)
+    v s,
+    (forall x, 
+      evalDist (c1a _ _ (randomFunc rndRange DomainRO_EqDec) s) x ==
+      evalDist (c1b _ _ (randomFunc rndRange DomainRO_EqDec) s) x) ->
+    (forall x1 s v,
+      evalDist (z <-$
+     (c2a x1)
+       (list (DomainRO * RangeRO))
+       (list_EqDec
+          (pair_EqDec DomainRO_EqDec RangeRO_EqDec))
+       (randomFunc rndRange DomainRO_EqDec) s;
+     [a, s]<-2 z; ret (f a s)) v ==
+     evalDist
+    (z <-$
+     (c2b x1)
+       (list (DomainRO * RangeRO))
+       (list_EqDec
+          (pair_EqDec DomainRO_EqDec RangeRO_EqDec))
+       (randomFunc rndRange DomainRO_EqDec) s;
+     [a, s]<-2 z; ret (f a s)) v
+    ) ->
+    evalDist (z <-$
+   (x1 <--$ c1a; c2a x1)
+     (list (DomainRO * RangeRO))
+     (list_EqDec
+        (pair_EqDec DomainRO_EqDec RangeRO_EqDec))
+     (randomFunc rndRange DomainRO_EqDec) s;
+   [a, s]<-2 z; ret (f a s)) v ==
+   evalDist
+  (z <-$
+   (x1 <--$ c1b; c2b x1)
+     (list (DomainRO * RangeRO))
+     (list_EqDec
+        (pair_EqDec DomainRO_EqDec RangeRO_EqDec))
+     (randomFunc rndRange DomainRO_EqDec) s;
+   [a, s]<-2 z; ret (f a s)) v.
+
+    intuition idtac.
+    Local Opaque evalDist.
+    simpl.
+    fcf_inline_first.
+    fcf_skip.
+    fcf_simp.
+    eauto.
+
+    Local Transparent evalDist.
+
+  Qed.
+
+  Theorem ExpROM_seq_eq : forall (A B : Set) 
+    (eqdb : EqDec B)
+    (c1a c1b : OracleComp DomainRO RangeRO A) 
+    (c2a c2b : A -> OracleComp DomainRO RangeRO B) 
+    v s,
+    (forall x, 
+      evalDist (c1a _ _ (randomFunc rndRange DomainRO_EqDec) s) x ==
+      evalDist (c1b _ _ (randomFunc rndRange DomainRO_EqDec) s) x) ->
+    (forall x1 s v,
+      evalDist (z <-$
+     (c2a x1)
+       (list (DomainRO * RangeRO))
+       (list_EqDec
+          (pair_EqDec DomainRO_EqDec RangeRO_EqDec))
+       (randomFunc rndRange DomainRO_EqDec) s;
+     [a, _]<-2 z; ret a) v ==
+     evalDist
+    (z <-$
+     (c2b x1)
+       (list (DomainRO * RangeRO))
+       (list_EqDec
+          (pair_EqDec DomainRO_EqDec RangeRO_EqDec))
+       (randomFunc rndRange DomainRO_EqDec) s;
+     [a, _]<-2 z; ret a) v
+    ) ->
+    evalDist (z <-$
+   (x1 <--$ c1a; c2a x1)
+     (list (DomainRO * RangeRO))
+     (list_EqDec
+        (pair_EqDec DomainRO_EqDec RangeRO_EqDec))
+     (randomFunc rndRange DomainRO_EqDec) s;
+   [a, _]<-2 z; ret a) v ==
+   evalDist
+  (z <-$
+   (x1 <--$ c1b; c2b x1)
+     (list (DomainRO * RangeRO))
+     (list_EqDec
+        (pair_EqDec DomainRO_EqDec RangeRO_EqDec))
+     (randomFunc rndRange DomainRO_EqDec) s;
+   [a, _]<-2 z; ret a) v.
+
+    intuition idtac.
+    Local Opaque evalDist.
+    simpl.
+    fcf_inline_first.
+    fcf_skip.
+    fcf_simp.
+    eauto.
+
+    Local Transparent evalDist.
+
+  Qed.
+
+  Theorem randomFunc_lookup_Some_inv : forall (D R : Set)(eqdd : EqDec D)(rndR : Comp R) s1 s2 v x b a,
+    In (v, s2) (getSupport (@randomFunc D R rndR _ s1 a)) ->
+    arrayLookup _ s1 x = Some b ->
+    arrayLookup _ s2 x = Some b.
+
+    intuition idtac.
+    unfold randomFunc in *.
+    case_eq (arrayLookup eqdd s1 a); intuition idtac;
+    rewrite H1 in H;
+    repeat simp_in_support.
+    trivial.
+    simpl.
+    case_eq (eqb x a); intuition idtac.
+    rewrite eqb_leibniz in H.
+    subst.
+    rewrite H0 in H1.
+    discriminate.
+
+  Qed.
+
+  (* If the function is a fold with a commutative accumulator, then independent statements
+  can be swapped. *)
+
+  Theorem sumList_permutation_body_eq:
+    forall (A : Set) (f1 f2 : A -> Rat) (ls1 ls2 : list A),
+    Permutation ls1 ls2 -> 
+    (forall a, In a ls2 -> (f1 a == f2 a)) ->
+    sumList ls1 f1 == sumList ls2 f2.
+
+    intros.
+    eapply eqRat_trans.
+    eapply sumList_permutation; eauto.
+    eapply sumList_body_eq; intuition idtac.
+
+  Qed.
+
+  Variable leDom : DomainRO -> DomainRO -> bool.
+  Hypothesis leDom_trans : forall a1 a2 a3, leDom a1 a2 = true -> leDom a2 a3 = true -> leDom a1 a3 = true.
+  Hypothesis leDom_refl : forall a, leDom a a = true.
+  Hypothesis leDom_antisymm : forall a1 a2, leDom a1 a2 = true -> leDom a2 a1 = true -> a1 = a2.
+  Hypothesis leDOm_total : forall a1 a2, (leDom a1 a2) || (leDom a2 a1) = true.
+
+  Theorem ExpROM_swap : forall (A B C : Set) 
+    (c1 : OracleComp DomainRO RangeRO A) 
+    (c2 : OracleComp DomainRO RangeRO B) 
+    (c3 : A -> B -> OracleComp DomainRO RangeRO C)
+    (E : Set)(eqde : EqDec E)(f2 : C -> E -> (DomainRO * RangeRO) -> E)
+    (init : E) s x,
+    (forall c e d1 d2, f2 c (f2 c e d1) d2 = f2 c (f2 c e d2) d1) ->
+    evalDist (ExpROM_gen_s (x1 <--$ c1; x2 <--$ c2; c3 x1 x2) _ (fun c ls => fold_left (fun e d => (f2 c e d)) ls init) s ) x ==
+    evalDist (ExpROM_gen_s (x2 <--$ c2; x1 <--$ c1; c3 x1 x2) _ (fun c ls => fold_left (fun e d => (f2 c e d)) ls init) s ) x.
+
+    intuition idtac.
+
+    assert RangeRO as RangeRO_ex.
+    eapply comp_base_exists; eauto.
+
+    assert A as a_ex.
+    eapply oc_base_exists; eauto.
+    
+    assert B as b_ex.
+    eapply oc_base_exists; eauto.
+
+    assert C as c_ex.
+    eapply oc_base_exists.
+    eapply c3; intuition idtac.
+    intuition idtac.
+
+    unfold ExpROM_gen_s.
+    
+    eapply (@eqRat_trans  _
+      (evalDist (z <-$
+     (x1 <--$ c1; x2 <--$ c2; c3 x1 x2)
+       (list (DomainRO * RangeRO))
+       (list_EqDec (pair_EqDec DomainRO_EqDec RangeRO_EqDec))
+       (sortedRandomFunc _ _ leDom rndRange) (sortDom leDom s);
+     [t, s0]<-2 z;
+     ret fold_left
+           (fun (e : E) (d : DomainRO * RangeRO) => f2 t e d)
+           s0 init) x)
+    ).
+
+    eapply comp_spec_eq_impl_eq.
+    fcf_skip.
+    eapply fcf_oracle_eq.
+    2:{
+    intros.
+    assert ((fun x1 x2 => x2 = sortDom leDom x1) x1 x2).
+    eapply H0.
+    simpl in *.
+    subst.
+    eapply sortedRandomFunc_sorted_equiv; intuition idtac.
+    }
+    simpl in *.
+    trivial.
+    simpl in *; intuition idtac.
+    destruct b0; simpl in *; subst.
+    eapply comp_spec_ret; intuition idtac.
+    eapply fold_left_comm_perm_eq; intuition idtac.
+    eapply sortDom_perm.
+    eauto.
+    symmetry.
+    eapply (@eqRat_trans  _
+      (evalDist (z <-$
+     (x1 <--$ c2; x2 <--$ c1; c3 x2 x1)
+       (list (DomainRO * RangeRO))
+       (list_EqDec (pair_EqDec DomainRO_EqDec RangeRO_EqDec))
+       (sortedRandomFunc _ _ leDom rndRange) (sortDom leDom s);
+     [t, s0]<-2 z;
+     ret fold_left
+           (fun (e : E) (d : DomainRO * RangeRO) => f2 t e d)
+           s0 init) x)
+    ).
+
+    eapply comp_spec_eq_impl_eq.
+    fcf_skip.
+    eapply fcf_oracle_eq.
+    2:{
+    intros.
+    assert ((fun x1 x2 => x2 = sortDom leDom x1) x1 x2).
+    eapply H0.
+    simpl in *.
+    subst.
+    eapply sortedRandomFunc_sorted_equiv; intuition idtac.
+    }
+    simpl in *.
+    trivial.
+    simpl in *; intuition idtac.
+    destruct b0; simpl in *; subst.
+    eapply comp_spec_ret; intuition idtac.
+    eapply fold_left_comm_perm_eq; intuition idtac.
+    eapply sortDom_perm.
+    eauto.
+
+    eapply comp_spec_eq_impl_eq.
+    simpl.
+    eapply (@comp_spec_eq_trans _ _ _
+      (z <-$
+     ([z, z2, s'0] <-$3 (z0 <-$
+      c2 (list (DomainRO * RangeRO))
+        (list_EqDec
+           (pair_EqDec DomainRO_EqDec
+              RangeRO_EqDec))
+        (sortedRandomFunc DomainRO_EqDec
+           RangeRO_EqDec leDom rndRange)
+        (sortDom leDom s);
+      [z, s']<-2 z0;
+      z1 <-$
+      c1 (list (DomainRO * RangeRO))
+        (list_EqDec
+           (pair_EqDec DomainRO_EqDec
+              RangeRO_EqDec))
+        (sortedRandomFunc DomainRO_EqDec
+           RangeRO_EqDec leDom rndRange) s';
+      [z2, s'0]<-2 z1;
+      ret (z, z2, s'0));
+
+      (c3 z2 z) (list (DomainRO * RangeRO))
+        (list_EqDec
+           (pair_EqDec DomainRO_EqDec
+              RangeRO_EqDec))
+        (sortedRandomFunc DomainRO_EqDec
+           RangeRO_EqDec leDom rndRange) s'0);
+     [t, s0]<-2 z;
+     ret fold_left
+           (fun (e : E) (d : DomainRO * RangeRO)
+            => f2 t e d) s0 init)
+    ).
+    fcf_inline_first.
+    fcf_skip.
+    fcf_inline_first.
+    fcf_skip.
+    fcf_simp.
+    eapply comp_spec_eq_refl.
+
+    eapply comp_spec_eq_symm.
+    eapply (@comp_spec_eq_trans _ _ _
+      (z <-$
+     ([z, z2, s'0] <-$3 (z0 <-$
+      c1 (list (DomainRO * RangeRO))
+        (list_EqDec
+           (pair_EqDec DomainRO_EqDec
+              RangeRO_EqDec))
+        (sortedRandomFunc DomainRO_EqDec
+           RangeRO_EqDec leDom rndRange)
+        (sortDom leDom s);
+      [z, s']<-2 z0;
+      z1 <-$
+      c2 (list (DomainRO * RangeRO))
+        (list_EqDec
+           (pair_EqDec DomainRO_EqDec
+              RangeRO_EqDec))
+        (sortedRandomFunc DomainRO_EqDec
+           RangeRO_EqDec leDom rndRange) s';
+      [z2, s'0]<-2 z1;
+      ret (z2, z, s'0));
+
+      (c3 z2 z) (list (DomainRO * RangeRO))
+        (list_EqDec
+           (pair_EqDec DomainRO_EqDec
+              RangeRO_EqDec))
+        (sortedRandomFunc DomainRO_EqDec
+           RangeRO_EqDec leDom rndRange) s'0);
+     [t, s0]<-2 z;
+     ret fold_left
+           (fun (e : E) (d : DomainRO * RangeRO)
+            => f2 t e d) s0 init)
+    ).
+    fcf_inline_first.
+    fcf_skip.
+    fcf_inline_first.
+    fcf_skip.
+    fcf_simp.
+    eapply comp_spec_eq_refl.
+
+    eapply comp_spec_seq_eq; trivial.
+    eapply comp_spec_seq_eq; trivial.
+    
+    intuition idtac.
+    intuition idtac.
+
+    eapply comp_spec_eq_symm.
+    eapply ExpROM_swap_spec; intuition idtac.
+    eapply sortedRandomFunc_swap; intuition idtac.
+    intuition idtac.
+    eapply comp_spec_eq_refl.
+    intuition idtac.
+    eapply comp_spec_eq_refl.
+
+    Unshelve.
+
+    eapply oc_EqDec.
+    eapply c3; intuition idtac.
+    intuition idtac.
+    intuition idtac.
+    
+    eapply oc_EqDec.
+    eapply c3; intuition idtac.
+    intuition idtac.
+    intuition idtac.
+
+    eapply pair_EqDec.
+    eapply oc_EqDec; eauto.
+    eapply list_EqDec.
+    eapply pair_EqDec; intuition idtac.
+
+    eapply pair_EqDec.
+    eapply oc_EqDec; eauto.
+    eapply list_EqDec.
+    eapply pair_EqDec; eauto.
+    
+    eapply pair_EqDec.
+    eapply oc_EqDec; eauto.
+    eapply list_EqDec.
+    eapply pair_EqDec; eauto.
+    
+    eapply pair_EqDec.
+    eapply oc_EqDec; eauto.
+    eapply list_EqDec.
+    eapply pair_EqDec; eauto.
+
+    eapply pair_EqDec.
+    eapply oc_EqDec; eauto.
+    eapply list_EqDec.
+    eapply pair_EqDec; eauto.
+    eapply oc_EqDec; eauto.
+    eapply oc_EqDec; eauto.
+  Qed.  
+    
+End ExperimentROM.
