src/FCF/RndListPred.v
@@ -1,0 +1,339 @@
+(* Some arguments about lists and random values. *)
+
+Require Import FCF.
+Require Import FCF.CompFold.
+Require Import FCF.RndInList.
+
+Set Implicit Arguments.
+Local Open Scope list_scope.
+
+Section RndListIn.
+
+  Variable A : Set.
+  Hypothesis eqda : EqDec A.
+  Variable c : Comp A. 
+  Variable a : A.
+  
+  Definition RndListIn_G (B : Type)(ls : list B) :=
+    x <-$ compMap _ (fun _ => c) ls;
+    ret (if (in_dec (EqDec_dec _) a x) then true else false).
+
+  Theorem RndListIn_Prob : forall (B : Type)(ls : list B), 
+    Pr[RndListIn_G ls] <= (length ls)/1 * (evalDist c a).
+
+    Local Opaque evalDist.
+
+    unfold RndListIn_G in *.
+    induction ls; intuition idtac; simpl in *.
+    comp_simp.
+    match goal with
+    | [|- context[if ?a then _ else _] ] => 
+      destruct a
+    end.
+    simpl in *.
+    intuition idtac.
+    rewrite evalDist_ret_0.
+    rattac.
+    intuition idtac; discriminate.
+    
+    simpl.
+    inline_first.
+    eapply leRat_trans.
+    eapply (evalDist_bind_event_le _ _ (fun z => eqb a z)).
+    reflexivity.
+    intuition idtac.
+    
+    assert (Pr 
+   [x <-$
+    (lsb' <-$ compMap _ (fun _ => c) ls;
+     ret (a1 :: lsb')%list);
+    ret (if in_dec (EqDec_dec _) a x then true else false)
+   ] ==
+            Pr 
+   [x <-$ compMap _ (fun _ => c) ls;
+    ret (if in_dec (EqDec_dec _) a x then true else false)
+   ]).
+
+    inline_first.
+    comp_skip.
+
+    match goal with
+    | [|- context[if ?a then _ else _] ] => 
+      destruct a
+    end.
+    simpl in *.
+    intuition idtac; subst.
+    rewrite eqb_refl in *.
+    discriminate.
+    match goal with
+    | [|- context[if ?a then _ else _] ] => 
+      destruct a
+    end.
+    reflexivity.
+    intuition idtac.
+    simpl in *.
+    intuition idtac.
+    match goal with
+    | [|- context[if ?a then _ else _] ] => 
+      destruct a
+    end.
+    intuition idtac.
+    reflexivity.
+
+    rewrite H1.
+    rewrite IHls.
+    reflexivity.
+
+    rewrite <- evalDist_event_equiv.
+    
+    eapply leRat_trans.
+    2:{
+      eapply eqRat_impl_leRat.
+      symmetry.
+      cutrewrite (S (length ls) = 1 + (length ls))%nat.
+      rewrite ratAdd_num.
+      rewrite ratMult_distrib_r.
+      reflexivity.
+      trivial.
+    }
+    eapply eqRat_impl_leRat.
+    rewrite ratMult_1_l.
+    reflexivity.
+
+    Local Transparent evalDist.
+
+  Qed.
+
+End RndListIn.
+
+Section RndListPred.
+
+  Variable A : Set.
+  Hypothesis eqda : EqDec A.
+  Variable c : Comp A. 
+  Variable f : A -> bool.
+
+  Definition RndListPred_G (B : Type)(ls : list B) :=
+    x <-$ compMap _ (fun _ => c) ls;
+    ret (any_dec f x).
+
+  Theorem RndListPred_Prob : forall (B : Type)(ls : list B), 
+    Pr[RndListPred_G ls] <= (length ls)/1 * Pr[x <-$c; ret (f x)].
+
+    Local Opaque evalDist.
+
+    unfold RndListPred_G in *.
+    induction ls; intuition idtac; simpl in *.
+    comp_simp.
+    unfold any_dec.
+    simpl.
+    rewrite evalDist_ret_0.
+    eapply rat0_le_all.
+    intuition idtac.
+    discriminate.
+    
+    inline_first.
+    eapply leRat_trans.
+    eapply (evalDist_bind_event_le _ _ f).
+    reflexivity.
+    intuition idtac.
+    
+    assert (Pr 
+   [x <-$
+    (lsb' <-$ compMap _ (fun _ => c) ls;
+     ret (a0 :: lsb')%list);
+      ret any_dec f x 
+   ] ==
+            Pr 
+   [x <-$ compMap _ (fun _ => c) ls;
+    ret any_dec f x 
+   ]).
+
+    inline_first.
+    comp_skip.
+
+    rewrite any_dec_cons.
+    eapply evalDist_ret_eq.
+    rewrite H0.
+    trivial.
+    rewrite H1.
+    eauto.
+    
+    eapply leRat_trans.
+    2:{
+      eapply eqRat_impl_leRat.
+      symmetry.
+      cutrewrite (S (length ls) = 1 + (length ls))%nat.
+      rewrite ratAdd_num.
+      rewrite ratMult_distrib_r.
+      reflexivity.
+      trivial.
+    }
+    eapply eqRat_impl_leRat.
+    rewrite ratMult_1_l.
+    reflexivity.
+
+    Local Transparent evalDist.
+
+  Qed.
+
+End RndListPred.
+
+Section RndInList.
+
+  Variable A : Set.
+  Hypothesis eqda : EqDec A.
+  Variable c : Comp A. 
+  Hypothesis c_wf : well_formed_comp c.
+  Variable r : Rat.
+  Hypothesis collProb : forall x,
+    evalDist c x <= r.
+  
+  Definition RndInList_G (a : list A) :=
+    x <-$ c; 
+    ret (if (in_dec (EqDec_dec _) x a) then true else false).
+
+  Theorem RndInList_Prob : forall (a : list A),
+    Pr[RndInList_G a] <= (length a)/1 * r.
+
+    Local Opaque evalDist.
+
+    unfold RndInList_G in *.
+    induction a; intuition idtac; simpl in *.
+    fcf_irr_l.
+    rewrite evalDist_ret_0.
+    eapply rat0_le_all.
+    intuition idtac.
+    discriminate.
+
+    eapply leRat_trans.
+    eapply (evalDist_bind_event_le _ _ (fun x => eqb a x || if (in_dec (EqDec_dec _) x a0) then true else false)).
+    rewrite evalDist_orb_le.
+    rewrite <- evalDist_event_equiv.
+    rewrite IHa.
+    rewrite collProb.
+    reflexivity.
+    intros.
+  
+    apply orb_false_elim in H0.
+    intuition idtac.
+    destruct (EqDec_dec eqda a a1).
+    subst.
+    rewrite eqb_refl in *.
+    discriminate.
+    destruct (in_dec (EqDec_dec eqda) a1 a0).
+    discriminate.
+    rewrite evalDist_ret_0.
+    eapply rat0_le_all.
+    intuition idtac.
+    discriminate.
+    rewrite <- ratAdd_0_r.
+    rewrite ratMult_comm.
+    rewrite ratMult_ratAdd_cd.
+    simpl.
+    rewrite ratMult_comm.
+    reflexivity.
+  Qed.
+
+End RndInList.
+
+Section DupList.
+
+  Variable A : Set.
+  Hypothesis eqda : EqDec A.
+  Variable c : Comp A. 
+  Hypothesis c_wf : well_formed_comp c.
+  Variable r : Rat.
+
+  Hypothesis collProb : 
+    forall a, evalDist c a <= r.
+  
+  Definition DupList_G (B : Type)(ls : list B) :=
+    x <-$ compMap _ (fun _ => c) ls;
+    ret (hasDup _ x).
+
+  Theorem DupList_Prob : forall (B : Type)(ls : list B), 
+    Pr[DupList_G ls] <= ((length ls) * (length ls))/1 * r.
+
+    Local Opaque evalDist.
+
+    unfold DupList_G in *.
+    induction ls; intuition idtac; simpl in *.
+    comp_simp.
+    simpl.
+    rewrite evalDist_ret_0.
+    eapply rat0_le_all.
+    intuition idtac.
+    discriminate.
+    
+    assert (Pr [x <-$
+    (b <-$ c;
+     lsb' <-$ compMap eqda (fun _ : B => c) ls;
+     ret b :: lsb'); ret hasDup eqda x ]
+      ==
+    Pr [lsb' <-$ compMap eqda (fun _ : B => c) ls;
+    a0 <-$ c;
+    ret hasDup eqda (a0 :: lsb')]
+    ).
+    fcf_swap rightc.
+    fcf_inline_first.
+    fcf_skip.
+    fcf_inline_first.
+    fcf_skip.
+
+    rewrite H.
+    clear H.
+
+    eapply leRat_trans.
+    eapply (evalDist_bind_event_le _ _ (fun z => hasDup _ z )).
+    eauto.
+    intros.
+    eapply (evalDist_bind_event_le _ _ (fun z => if (in_dec (EqDec_dec _) z a0) then true else false )).
+    specialize (@RndInList_Prob _ _ c c_wf r collProb a0); intros.
+    unfold RndInList_G in *.
+    rewrite H1.
+    apply compMap_length in H.
+    rewrite H.
+    reflexivity.
+    intros.
+    simpl.
+    destruct (in_dec (EqDec_dec eqda) a1 a0).
+    discriminate.
+    rewrite H0.
+    rewrite evalDist_ret_0.
+    reflexivity.
+    intuition idtac.
+    discriminate.
+
+    rewrite <- ratAdd_0_r.
+    eapply leRat_trans.
+    2:{
+    eapply ratMult_leRat_compat.
+    eapply leRat_terms.
+    eapply Nat.le_succ_diag_r.
+    reflexivity.
+    reflexivity.
+    }
+    eapply leRat_trans.
+    2:{
+    eapply eqRat_impl_leRat.
+    symmetry.
+    rewrite ratAdd_den_same.
+    rewrite ratMult_distrib_r.
+    reflexivity.
+    }
+    rewrite ratAdd_comm.
+    eapply ratAdd_leRat_compat.
+    reflexivity.
+    eapply ratMult_leRat_compat.
+    eapply leRat_terms.
+    eapply mult_le_compat.
+    trivial.  
+    omega.
+    trivial.
+    reflexivity.
+
+    Local Transparent evalDist.
+  Qed.
+
+End DupList.
